fix the definition of OclAllInstances Instead of receiving as argument a lazy function, we replace it by a lifted version that could return None .
git-svn-id: https://projects.brucker.ch/hol-testgen/svn/HOL-TestGen/trunk/hol-testgen@9799 3260e6d1-4efc-4170-b0a7-36055960796d

examples/Employee_DesignModel_UMLPart.thy
@@ -1,5 +1,5 @@
 (*****************************************************************************
- * Featherweight-OCL --- A Formal Semantics for UML-OCL Version OCL 2.4 
+ * Featherweight-OCL --- A Formal Semantics for UML-OCL Version OCL 2.4
  *                       for the OMG Standard.
  *                       http://www.brucker.ch/projects/hol-testgen/
  *
@@ -122,8 +122,25 @@ where "Person (in\<^isub>o\<^isub>c\<^isub>l\<^isub>a\<^isub>n\<^isub>y(mk\<^isu
     | "Person (in\<^isub>p\<^isub>e\<^isub>r\<^isub>s\<^isub>o\<^isub>n(mk\<^isub>p\<^isub>e\<^isub>r\<^isub>s\<^isub>o\<^isub>n oid a b)) = mk\<^isub>p\<^isub>e\<^isub>r\<^isub>s\<^isub>o\<^isub>n oid a b"
 
 fun    OclAny :: "\<AA> \<Rightarrow> oclany"
-where "OclAny (in\<^isub>o\<^isub>c\<^isub>l\<^isub>a\<^isub>n\<^isub>y(X)) = X"
-     |"OclAny (in\<^isub>p\<^isub>e\<^isub>r\<^isub>s\<^isub>o\<^isub>n(mk\<^isub>p\<^isub>e\<^isub>r\<^isub>s\<^isub>o\<^isub>n oid a b)) = (mk\<^isub>o\<^isub>c\<^isub>l\<^isub>a\<^isub>n\<^isub>y oid \<lfloor>(a,b)\<rfloor>)"
+where "OclAny (in\<^isub>o\<^isub>c\<^isub>l\<^isub>a\<^isub>n\<^isub>y X) = X"
+     |"OclAny (in\<^isub>p\<^isub>e\<^isub>r\<^isub>s\<^isub>o\<^isub>n (mk\<^isub>p\<^isub>e\<^isub>r\<^isub>s\<^isub>o\<^isub>n oid a b)) = mk\<^isub>o\<^isub>c\<^isub>l\<^isub>a\<^isub>n\<^isub>y oid \<lfloor>(a,b)\<rfloor>"
+
+definition    Person' :: "\<AA> \<Rightarrow> person option"
+where "Person' = (\<lambda>x. case x of
+      in\<^isub>o\<^isub>c\<^isub>l\<^isub>a\<^isub>n\<^isub>y (mk\<^isub>o\<^isub>c\<^isub>l\<^isub>a\<^isub>n\<^isub>y oid \<lfloor>(a,b)\<rfloor>) \<Rightarrow> \<lfloor>mk\<^isub>p\<^isub>e\<^isub>r\<^isub>s\<^isub>o\<^isub>n oid a b\<rfloor>
+    | in\<^isub>p\<^isub>e\<^isub>r\<^isub>s\<^isub>o\<^isub>n (mk\<^isub>p\<^isub>e\<^isub>r\<^isub>s\<^isub>o\<^isub>n oid a b) \<Rightarrow> \<lfloor>mk\<^isub>p\<^isub>e\<^isub>r\<^isub>s\<^isub>o\<^isub>n oid a b\<rfloor>
+    | _ \<Rightarrow> None)"
+
+definition    OclAny' :: "\<AA> \<Rightarrow> oclany option"
+where "OclAny' = (\<lambda>x. case x of
+      in\<^isub>o\<^isub>c\<^isub>l\<^isub>a\<^isub>n\<^isub>y X \<Rightarrow> \<lfloor>X\<rfloor>
+    | in\<^isub>p\<^isub>e\<^isub>r\<^isub>s\<^isub>o\<^isub>n (mk\<^isub>p\<^isub>e\<^isub>r\<^isub>s\<^isub>o\<^isub>n oid a b) \<Rightarrow> \<lfloor>mk\<^isub>o\<^isub>c\<^isub>l\<^isub>a\<^isub>n\<^isub>y oid \<lfloor>(a,b)\<rfloor>\<rfloor>)"
+
+lemma oclany_none: "OclAny' x \<noteq> None"
+ apply(simp add: OclAny'_def)
+ apply(case_tac x, simp_all)
+ apply(case_tac person, simp_all)
+done
 
 (* PROBLEM: THIS CONSTRUCTION IS NO LONGER injective, thus invertible ...
    Maybe this causes BIG PROBLEMS for our entire construction of allInstances ... bu *)
@@ -208,6 +225,10 @@ lemma "Person .oclAllInstances() =
              (\<lambda>\<tau>.  Abs_Set_0 \<lfloor>\<lfloor>(Some \<circ> Some \<circ> Person_sumC)`(ran(heap(snd \<tau>))) \<rfloor>\<rfloor>) "
 by(rule ext, simp add:allinstances_def Person_def)
 
+lemma "allinstances' Person' =
+             (\<lambda>\<tau>.  Abs_Set_0  \<lfloor>\<lfloor>Some ` (Person' ` ran (heap (snd \<tau>)) - {None})\<rfloor>\<rfloor>) "
+by(rule ext, simp add:allinstances'_def)
+
 lemma "Person .oclAllInstances@pre() = 
              (\<lambda>\<tau>.  Abs_Set_0 \<lfloor>\<lfloor>(Some \<circ> Some \<circ> Person_sumC)`(ran(heap(fst \<tau>))) \<rfloor>\<rfloor>) "
 by(rule ext, simp add:allinstancesATpre_def Person_def)
@@ -215,6 +236,21 @@ by(rule ext, simp add:allinstancesATpre_def Person_def)
 lemma "OclAny .oclAllInstances() =
              (\<lambda>\<tau>.  Abs_Set_0 \<lfloor>\<lfloor>(Some \<circ> Some \<circ> OclAny_sumC)`(ran(heap(snd \<tau>))) \<rfloor>\<rfloor>) "
 by(rule ext, simp add:allinstances_def OclAny_def)
+
+lemma "allinstances' OclAny' =
+             (\<lambda>\<tau>.  Abs_Set_0  \<lfloor>\<lfloor> Some ` OclAny' ` ran (heap (snd \<tau>)) \<rfloor>\<rfloor>) "
+ apply(rule ext, simp add: allinstances'_def)
+ apply(subgoal_tac " (OclAny' ` ran (heap (snd \<tau>)) - {None}) = (OclAny' ` ran (heap (snd \<tau>)))", simp)
+ apply(simp add: image_def)
+ apply(rule equalityI)
+ apply(rule subsetI)
+ apply (metis (lifting) Diff_iff)
+ apply(rule subsetI)
+ apply(simp)
+ apply(drule bexE) prefer 2 apply assumption
+ apply(case_tac x, metis oclany_none)
+ apply(blast)
+done
 
 lemma "OclAny .oclAllInstances@pre() = 
              (\<lambda>\<tau>.  Abs_Set_0 \<lfloor>\<lfloor>(Some \<circ> Some \<circ> OclAny_sumC)`(ran(heap(fst \<tau>))) \<rfloor>\<rfloor>) "
@@ -773,17 +809,14 @@ by(auto simp: \<sigma>\<^isub>1_def)
 lemma [code_unfold]: "dom (heap \<sigma>\<^isub>1') = {oid\<^isub>1,oid\<^isub>2,oid\<^isub>3,oid\<^isub>4,(*,oid\<^isub>5*)oid\<^isub>6,oid\<^isub>7,oid\<^isub>8}"
 by(auto simp: \<sigma>\<^isub>1'_def)
 
-definition "X\<^isub>P\<^isub>e\<^isub>r\<^isub>s\<^isub>o\<^isub>n1 :: Person
-                   \<equiv> \<lambda> _ .\<lfloor>\<lfloor> person1 \<rfloor>\<rfloor>"
-definition "X\<^isub>P\<^isub>e\<^isub>r\<^isub>s\<^isub>o\<^isub>n2 \<equiv> \<lambda> _ .\<lfloor>\<lfloor> person2 \<rfloor>\<rfloor>"
-definition "X\<^isub>P\<^isub>e\<^isub>r\<^isub>s\<^isub>o\<^isub>n3 \<equiv> \<lambda> _ .\<lfloor>\<lfloor> person3 \<rfloor>\<rfloor>"
-definition "X\<^isub>P\<^isub>e\<^isub>r\<^isub>s\<^isub>o\<^isub>n4 \<equiv> \<lambda> _ .\<lfloor>\<lfloor> person4 \<rfloor>\<rfloor>"
-definition "X\<^isub>P\<^isub>e\<^isub>r\<^isub>s\<^isub>o\<^isub>n5 \<equiv> \<lambda> _ .\<lfloor>\<lfloor> person5 \<rfloor>\<rfloor>"
-definition "X\<^isub>P\<^isub>e\<^isub>r\<^isub>s\<^isub>o\<^isub>n6 \<equiv> \<lambda> _ .\<lfloor>\<lfloor> person6 \<rfloor>\<rfloor>"
-definition "X\<^isub>P\<^isub>e\<^isub>r\<^isub>s\<^isub>o\<^isub>n7 :: OclAny 
-                   \<equiv> \<lambda> _ .\<lfloor>\<lfloor> person7 \<rfloor>\<rfloor>"
-definition "X\<^isub>P\<^isub>e\<^isub>r\<^isub>s\<^isub>o\<^isub>n8 :: OclAny 
-                   \<equiv> \<lambda> _ .\<lfloor>\<lfloor> person8 \<rfloor>\<rfloor>"
+definition "X\<^isub>P\<^isub>e\<^isub>r\<^isub>s\<^isub>o\<^isub>n1 :: Person \<equiv> \<lambda> _ .\<lfloor>\<lfloor> person1 \<rfloor>\<rfloor>"
+definition "X\<^isub>P\<^isub>e\<^isub>r\<^isub>s\<^isub>o\<^isub>n2 :: Person \<equiv> \<lambda> _ .\<lfloor>\<lfloor> person2 \<rfloor>\<rfloor>"
+definition "X\<^isub>P\<^isub>e\<^isub>r\<^isub>s\<^isub>o\<^isub>n3 :: Person \<equiv> \<lambda> _ .\<lfloor>\<lfloor> person3 \<rfloor>\<rfloor>"
+definition "X\<^isub>P\<^isub>e\<^isub>r\<^isub>s\<^isub>o\<^isub>n4 :: Person \<equiv> \<lambda> _ .\<lfloor>\<lfloor> person4 \<rfloor>\<rfloor>"
+definition "X\<^isub>P\<^isub>e\<^isub>r\<^isub>s\<^isub>o\<^isub>n5 :: Person \<equiv> \<lambda> _ .\<lfloor>\<lfloor> person5 \<rfloor>\<rfloor>"
+definition "X\<^isub>P\<^isub>e\<^isub>r\<^isub>s\<^isub>o\<^isub>n6 :: Person \<equiv> \<lambda> _ .\<lfloor>\<lfloor> person6 \<rfloor>\<rfloor>"
+definition "X\<^isub>P\<^isub>e\<^isub>r\<^isub>s\<^isub>o\<^isub>n7 :: OclAny \<equiv> \<lambda> _ .\<lfloor>\<lfloor> person7 \<rfloor>\<rfloor>"
+definition "X\<^isub>P\<^isub>e\<^isub>r\<^isub>s\<^isub>o\<^isub>n8 :: OclAny \<equiv> \<lambda> _ .\<lfloor>\<lfloor> person8 \<rfloor>\<rfloor>"
 
 lemma [code_unfold]: "((x::Person) \<doteq> y) = gen_ref_eq x y" by(simp only: StrictRefEq\<^isub>p\<^isub>e\<^isub>r\<^isub>s\<^isub>o\<^isub>n)
 
@@ -989,6 +1022,170 @@ proof -
                   person1_def person2_def person3_def person4_def person5_def person6_def person7_def person8_def)
  done
 qed
+
+lemma "\<And>\<sigma>\<^isub>1.    (\<sigma>\<^isub>1,\<sigma>\<^isub>1') \<Turnstile>      (allinstances' Person' \<doteq> Set{ X\<^isub>P\<^isub>e\<^isub>r\<^isub>s\<^isub>o\<^isub>n1, X\<^isub>P\<^isub>e\<^isub>r\<^isub>s\<^isub>o\<^isub>n2, X\<^isub>P\<^isub>e\<^isub>r\<^isub>s\<^isub>o\<^isub>n3, X\<^isub>P\<^isub>e\<^isub>r\<^isub>s\<^isub>o\<^isub>n4(*, X\<^isub>P\<^isub>e\<^isub>r\<^isub>s\<^isub>o\<^isub>n5*), X\<^isub>P\<^isub>e\<^isub>r\<^isub>s\<^isub>o\<^isub>n6, X\<^isub>P\<^isub>e\<^isub>r\<^isub>s\<^isub>o\<^isub>n7 .oclAsType(Person) })"
+proof -
+ have p0 : "\<And>S oid\<^isub>8 oid\<^isub>7 person8 person7. oid\<^isub>8 \<noteq> oid\<^isub>7 \<Longrightarrow>
+            S (oid\<^isub>8 \<mapsto> person8) (oid\<^isub>7 \<mapsto> person7) = S (oid\<^isub>7 \<mapsto> person7) (oid\<^isub>8 \<mapsto> person8)"
+ by (metis fun_upd_twist)
+
+ have perm : "\<sigma>\<^isub>1' = \<lparr> heap = empty
+                           (oid\<^isub>8 \<mapsto> in\<^isub>o\<^isub>c\<^isub>l\<^isub>a\<^isub>n\<^isub>y person8)
+                           (oid\<^isub>7 \<mapsto> in\<^isub>o\<^isub>c\<^isub>l\<^isub>a\<^isub>n\<^isub>y person7)
+                           (oid\<^isub>6 \<mapsto> in\<^isub>p\<^isub>e\<^isub>r\<^isub>s\<^isub>o\<^isub>n person6)
+                          (*oid\<^isub>5*)
+                           (oid\<^isub>4 \<mapsto> in\<^isub>p\<^isub>e\<^isub>r\<^isub>s\<^isub>o\<^isub>n person4)
+                           (oid\<^isub>3 \<mapsto> in\<^isub>p\<^isub>e\<^isub>r\<^isub>s\<^isub>o\<^isub>n person3)
+                           (oid\<^isub>2 \<mapsto> in\<^isub>p\<^isub>e\<^isub>r\<^isub>s\<^isub>o\<^isub>n person2)
+                           (oid\<^isub>1 \<mapsto> in\<^isub>p\<^isub>e\<^isub>r\<^isub>s\<^isub>o\<^isub>n person1)
+                , assocs = empty \<rparr>"
+  apply(simp add: \<sigma>\<^isub>1'_def
+                  oid\<^isub>1_def oid\<^isub>2_def oid\<^isub>3_def oid\<^isub>4_def oid\<^isub>5_def oid\<^isub>6_def oid\<^isub>7_def oid\<^isub>8_def)
+  apply(subst (1) p0, simp)
+  apply(subst (2) p0, simp) apply(subst (1) p0, simp)
+  apply(subst (3) p0, simp) apply(subst (2) p0, simp) apply(subst (1) p0, simp)
+  apply(subst (4) p0, simp) apply(subst (3) p0, simp) apply(subst (2) p0, simp) apply(subst (1) p0, simp)
+  apply(subst (5) p0, simp) apply(subst (4) p0, simp) apply(subst (3) p0, simp) apply(subst (2) p0, simp) apply(subst (1) p0, simp)
+  apply(subst (6) p0, simp) apply(subst (5) p0, simp) apply(subst (4) p0, simp) apply(subst (3) p0, simp) apply(subst (2) p0, simp) apply(subst (1) p0, simp)
+ by(simp)
+
+ fix \<sigma>\<^isub>1
+ have eq : "allinstances' Person' (\<sigma>\<^isub>1,\<sigma>\<^isub>1') =
+       Set{X\<^isub>P\<^isub>e\<^isub>r\<^isub>s\<^isub>o\<^isub>n1, X\<^isub>P\<^isub>e\<^isub>r\<^isub>s\<^isub>o\<^isub>n2, X\<^isub>P\<^isub>e\<^isub>r\<^isub>s\<^isub>o\<^isub>n3, X\<^isub>P\<^isub>e\<^isub>r\<^isub>s\<^isub>o\<^isub>n4(*, X\<^isub>P\<^isub>e\<^isub>r\<^isub>s\<^isub>o\<^isub>n5*), X\<^isub>P\<^isub>e\<^isub>r\<^isub>s\<^isub>o\<^isub>n6, X\<^isub>P\<^isub>e\<^isub>r\<^isub>s\<^isub>o\<^isub>n7 .oclAsType(Person)} (\<sigma>\<^isub>1,\<sigma>\<^isub>1')"
+  apply(simp only: perm)
+  apply(simp add: oid\<^isub>1_def oid\<^isub>2_def oid\<^isub>3_def oid\<^isub>4_def oid\<^isub>5_def oid\<^isub>6_def oid\<^isub>7_def oid\<^isub>8_def
+                  X\<^isub>P\<^isub>e\<^isub>r\<^isub>s\<^isub>o\<^isub>n1_def X\<^isub>P\<^isub>e\<^isub>r\<^isub>s\<^isub>o\<^isub>n2_def X\<^isub>P\<^isub>e\<^isub>r\<^isub>s\<^isub>o\<^isub>n3_def X\<^isub>P\<^isub>e\<^isub>r\<^isub>s\<^isub>o\<^isub>n4_def X\<^isub>P\<^isub>e\<^isub>r\<^isub>s\<^isub>o\<^isub>n5_def X\<^isub>P\<^isub>e\<^isub>r\<^isub>s\<^isub>o\<^isub>n6_def X\<^isub>P\<^isub>e\<^isub>r\<^isub>s\<^isub>o\<^isub>n7_def X\<^isub>P\<^isub>e\<^isub>r\<^isub>s\<^isub>o\<^isub>n8_def)
+  apply(subst state_update_vs_allInstances'_rec, simp, simp add: Person'_def
+   person1_def person2_def person3_def person4_def person5_def person6_def person7_def person8_def)
+  apply(subst state_update_vs_allInstances'_rec, simp, simp add: Person'_def
+   person1_def person2_def person3_def person4_def person5_def person6_def person7_def person8_def)
+  apply(subst state_update_vs_allInstances'_rec, simp, simp add: Person'_def
+   person1_def person2_def person3_def person4_def person5_def person6_def person7_def person8_def)
+  apply(subst state_update_vs_allInstances'_rec, simp, simp add: Person'_def
+   person1_def person2_def person3_def person4_def person5_def person6_def person7_def person8_def)
+  apply(subst state_update_vs_allInstances'_rec, simp, simp add: Person'_def
+   person1_def person2_def person3_def person4_def person5_def person6_def person7_def person8_def)
+  apply(subst state_update_vs_allInstances'_rec, simp, simp add: Person'_def
+   person1_def person2_def person3_def person4_def person5_def person6_def person7_def person8_def)
+  apply(subst state_update_vs_allInstances'_recnone, simp, simp add: Person'_def
+   person1_def person2_def person3_def person4_def person5_def person6_def person7_def person8_def)
+  apply(subst state_update_vs_allInstances'_rec0)
+
+  apply(subst including_cp_all
+                                         ) prefer 4 apply(subst cp_OclIncluding[symmetric])
+  apply(subst including_cp_all[of _ _ _ "(\<sigma>\<^isub>1, \<lparr>heap = [7 \<mapsto> in\<^isub>o\<^isub>c\<^isub>l\<^isub>a\<^isub>n\<^isub>y person8],
+                    assocs = Map.empty\<rparr>)"]) prefer 4 apply(subst cp_OclIncluding[symmetric])
+  apply(subst including_cp_all[of _ _ _ "(\<sigma>\<^isub>1, \<lparr>heap = [7 \<mapsto> in\<^isub>o\<^isub>c\<^isub>l\<^isub>a\<^isub>n\<^isub>y person8, 6 \<mapsto> in\<^isub>o\<^isub>c\<^isub>l\<^isub>a\<^isub>n\<^isub>y person7],
+                    assocs = Map.empty\<rparr>)"]) prefer 4 apply(subst cp_OclIncluding[symmetric])
+  apply(subst including_cp_all[of _ _ _ "(\<sigma>\<^isub>1, \<lparr>heap = [7 \<mapsto> in\<^isub>o\<^isub>c\<^isub>l\<^isub>a\<^isub>n\<^isub>y person8, 6 \<mapsto> in\<^isub>o\<^isub>c\<^isub>l\<^isub>a\<^isub>n\<^isub>y person7, 5 \<mapsto> in\<^isub>p\<^isub>e\<^isub>r\<^isub>s\<^isub>o\<^isub>n person6],
+                    assocs = Map.empty\<rparr>)"]) prefer 4 apply(subst cp_OclIncluding[symmetric])
+  apply(subst including_cp_all[of _ _ _ "(\<sigma>\<^isub>1, \<lparr>heap = [7 \<mapsto> in\<^isub>o\<^isub>c\<^isub>l\<^isub>a\<^isub>n\<^isub>y person8, 6 \<mapsto> in\<^isub>o\<^isub>c\<^isub>l\<^isub>a\<^isub>n\<^isub>y person7, 5 \<mapsto> in\<^isub>p\<^isub>e\<^isub>r\<^isub>s\<^isub>o\<^isub>n person6, 3 \<mapsto> in\<^isub>p\<^isub>e\<^isub>r\<^isub>s\<^isub>o\<^isub>n person4],
+                    assocs = Map.empty\<rparr>)"]) prefer 4 apply(subst cp_OclIncluding[symmetric])
+  apply(subst including_cp_all[of _ _ _ "(\<sigma>\<^isub>1, \<lparr>heap = [7 \<mapsto> in\<^isub>o\<^isub>c\<^isub>l\<^isub>a\<^isub>n\<^isub>y person8, 6 \<mapsto> in\<^isub>o\<^isub>c\<^isub>l\<^isub>a\<^isub>n\<^isub>y person7, 5 \<mapsto> in\<^isub>p\<^isub>e\<^isub>r\<^isub>s\<^isub>o\<^isub>n person6, 3 \<mapsto> in\<^isub>p\<^isub>e\<^isub>r\<^isub>s\<^isub>o\<^isub>n person4, 2 \<mapsto> in\<^isub>p\<^isub>e\<^isub>r\<^isub>s\<^isub>o\<^isub>n person3],
+                    assocs = Map.empty\<rparr>)"]) prefer 4 apply(subst cp_OclIncluding[symmetric])
+  apply(subst including_cp_all[of _ _ _ "(\<sigma>\<^isub>1, \<lparr>heap = [7 \<mapsto> in\<^isub>o\<^isub>c\<^isub>l\<^isub>a\<^isub>n\<^isub>y person8, 6 \<mapsto> in\<^isub>o\<^isub>c\<^isub>l\<^isub>a\<^isub>n\<^isub>y person7, 5 \<mapsto> in\<^isub>p\<^isub>e\<^isub>r\<^isub>s\<^isub>o\<^isub>n person6, 3 \<mapsto> in\<^isub>p\<^isub>e\<^isub>r\<^isub>s\<^isub>o\<^isub>n person4, 2 \<mapsto> in\<^isub>p\<^isub>e\<^isub>r\<^isub>s\<^isub>o\<^isub>n person3, Suc 0 \<mapsto> in\<^isub>p\<^isub>e\<^isub>r\<^isub>s\<^isub>o\<^isub>n person2],
+                    assocs = Map.empty\<rparr>)"]) prefer 4 apply(subst cp_OclIncluding[symmetric])
+  apply(subst including_cp_all[of _ _ _ "(\<sigma>\<^isub>1, \<lparr>heap = [7 \<mapsto> in\<^isub>o\<^isub>c\<^isub>l\<^isub>a\<^isub>n\<^isub>y person8, 6 \<mapsto> in\<^isub>o\<^isub>c\<^isub>l\<^isub>a\<^isub>n\<^isub>y person7, 5 \<mapsto> in\<^isub>p\<^isub>e\<^isub>r\<^isub>s\<^isub>o\<^isub>n person6, 3 \<mapsto> in\<^isub>p\<^isub>e\<^isub>r\<^isub>s\<^isub>o\<^isub>n person4, 2 \<mapsto> in\<^isub>p\<^isub>e\<^isub>r\<^isub>s\<^isub>o\<^isub>n person3, Suc 0 \<mapsto> in\<^isub>p\<^isub>e\<^isub>r\<^isub>s\<^isub>o\<^isub>n person2, 0 \<mapsto> in\<^isub>p\<^isub>e\<^isub>r\<^isub>s\<^isub>o\<^isub>n person1],
+                    assocs = Map.empty\<rparr>)"]) prefer 4 apply(subst cp_OclIncluding[symmetric])
+
+  apply(simp add: Person'_def person1_def person2_def person3_def person4_def person5_def person6_def person7_def person8_def)
+  apply(simp_all add: is_int_def)
+  apply((rule including_cp_all, simp_all add: is_int_def)+, simp add: mtSet_def)+
+  apply(simp add: mtSet_def) apply(simp add: mtSet_def) apply(simp add: mtSet_def)
+ by (metis (no_types) foundation1 foundation16 mtSet_defined)
+
+ show "?thesis \<sigma>\<^isub>1"
+  apply(simp only: StrictRefEq_set StrongEq_def true_def OclValid_def)
+  apply(subst cp_valid)
+  apply(subst (1 2) eq)
+  apply(subst cp_valid[symmetric])
+  apply(simp add: X\<^isub>P\<^isub>e\<^isub>r\<^isub>s\<^isub>o\<^isub>n1_def X\<^isub>P\<^isub>e\<^isub>r\<^isub>s\<^isub>o\<^isub>n2_def X\<^isub>P\<^isub>e\<^isub>r\<^isub>s\<^isub>o\<^isub>n3_def X\<^isub>P\<^isub>e\<^isub>r\<^isub>s\<^isub>o\<^isub>n4_def X\<^isub>P\<^isub>e\<^isub>r\<^isub>s\<^isub>o\<^isub>n5_def X\<^isub>P\<^isub>e\<^isub>r\<^isub>s\<^isub>o\<^isub>n6_def X\<^isub>P\<^isub>e\<^isub>r\<^isub>s\<^isub>o\<^isub>n7_def X\<^isub>P\<^isub>e\<^isub>r\<^isub>s\<^isub>o\<^isub>n8_def
+                  person1_def person2_def person3_def person4_def person5_def person6_def person7_def person8_def)
+ done
+qed
+
+lemma "\<And>\<sigma>\<^isub>1.    (\<sigma>\<^isub>1,\<sigma>\<^isub>1') \<Turnstile>      (allinstances' OclAny' \<doteq> Set{ X\<^isub>P\<^isub>e\<^isub>r\<^isub>s\<^isub>o\<^isub>n1 .oclAsType(OclAny), X\<^isub>P\<^isub>e\<^isub>r\<^isub>s\<^isub>o\<^isub>n2 .oclAsType(OclAny), X\<^isub>P\<^isub>e\<^isub>r\<^isub>s\<^isub>o\<^isub>n3 .oclAsType(OclAny), X\<^isub>P\<^isub>e\<^isub>r\<^isub>s\<^isub>o\<^isub>n4 .oclAsType(OclAny)(*, X\<^isub>P\<^isub>e\<^isub>r\<^isub>s\<^isub>o\<^isub>n5*), X\<^isub>P\<^isub>e\<^isub>r\<^isub>s\<^isub>o\<^isub>n6 .oclAsType(OclAny), X\<^isub>P\<^isub>e\<^isub>r\<^isub>s\<^isub>o\<^isub>n7, X\<^isub>P\<^isub>e\<^isub>r\<^isub>s\<^isub>o\<^isub>n8 })"
+proof -
+ have p0 : "\<And>S oid\<^isub>8 oid\<^isub>7 person8 person7. oid\<^isub>8 \<noteq> oid\<^isub>7 \<Longrightarrow>
+            S (oid\<^isub>8 \<mapsto> person8) (oid\<^isub>7 \<mapsto> person7) = S (oid\<^isub>7 \<mapsto> person7) (oid\<^isub>8 \<mapsto> person8)"
+ by (metis fun_upd_twist)
+
+ have perm : "\<sigma>\<^isub>1' = \<lparr> heap = empty
+                           (oid\<^isub>8 \<mapsto> in\<^isub>o\<^isub>c\<^isub>l\<^isub>a\<^isub>n\<^isub>y person8)
+                           (oid\<^isub>7 \<mapsto> in\<^isub>o\<^isub>c\<^isub>l\<^isub>a\<^isub>n\<^isub>y person7)
+                           (oid\<^isub>6 \<mapsto> in\<^isub>p\<^isub>e\<^isub>r\<^isub>s\<^isub>o\<^isub>n person6)
+                          (*oid\<^isub>5*)
+                           (oid\<^isub>4 \<mapsto> in\<^isub>p\<^isub>e\<^isub>r\<^isub>s\<^isub>o\<^isub>n person4)
+                           (oid\<^isub>3 \<mapsto> in\<^isub>p\<^isub>e\<^isub>r\<^isub>s\<^isub>o\<^isub>n person3)
+                           (oid\<^isub>2 \<mapsto> in\<^isub>p\<^isub>e\<^isub>r\<^isub>s\<^isub>o\<^isub>n person2)
+                           (oid\<^isub>1 \<mapsto> in\<^isub>p\<^isub>e\<^isub>r\<^isub>s\<^isub>o\<^isub>n person1)
+                , assocs = empty \<rparr>"
+  apply(simp add: \<sigma>\<^isub>1'_def
+                  oid\<^isub>1_def oid\<^isub>2_def oid\<^isub>3_def oid\<^isub>4_def oid\<^isub>5_def oid\<^isub>6_def oid\<^isub>7_def oid\<^isub>8_def)
+  apply(subst (1) p0, simp)
+  apply(subst (2) p0, simp) apply(subst (1) p0, simp)
+  apply(subst (3) p0, simp) apply(subst (2) p0, simp) apply(subst (1) p0, simp)
+  apply(subst (4) p0, simp) apply(subst (3) p0, simp) apply(subst (2) p0, simp) apply(subst (1) p0, simp)
+  apply(subst (5) p0, simp) apply(subst (4) p0, simp) apply(subst (3) p0, simp) apply(subst (2) p0, simp) apply(subst (1) p0, simp)
+  apply(subst (6) p0, simp) apply(subst (5) p0, simp) apply(subst (4) p0, simp) apply(subst (3) p0, simp) apply(subst (2) p0, simp) apply(subst (1) p0, simp)
+ by(simp)
+
+ fix \<sigma>\<^isub>1
+ have eq : "allinstances' OclAny' (\<sigma>\<^isub>1,\<sigma>\<^isub>1') =
+       Set{ X\<^isub>P\<^isub>e\<^isub>r\<^isub>s\<^isub>o\<^isub>n1 .oclAsType(OclAny), X\<^isub>P\<^isub>e\<^isub>r\<^isub>s\<^isub>o\<^isub>n2 .oclAsType(OclAny), X\<^isub>P\<^isub>e\<^isub>r\<^isub>s\<^isub>o\<^isub>n3 .oclAsType(OclAny), X\<^isub>P\<^isub>e\<^isub>r\<^isub>s\<^isub>o\<^isub>n4 .oclAsType(OclAny)(*, X\<^isub>P\<^isub>e\<^isub>r\<^isub>s\<^isub>o\<^isub>n5*), X\<^isub>P\<^isub>e\<^isub>r\<^isub>s\<^isub>o\<^isub>n6 .oclAsType(OclAny), X\<^isub>P\<^isub>e\<^isub>r\<^isub>s\<^isub>o\<^isub>n7, X\<^isub>P\<^isub>e\<^isub>r\<^isub>s\<^isub>o\<^isub>n8 } (\<sigma>\<^isub>1,\<sigma>\<^isub>1')"
+  apply(simp only: perm)
+  apply(simp add: oid\<^isub>1_def oid\<^isub>2_def oid\<^isub>3_def oid\<^isub>4_def oid\<^isub>5_def oid\<^isub>6_def oid\<^isub>7_def oid\<^isub>8_def
+                  X\<^isub>P\<^isub>e\<^isub>r\<^isub>s\<^isub>o\<^isub>n1_def X\<^isub>P\<^isub>e\<^isub>r\<^isub>s\<^isub>o\<^isub>n2_def X\<^isub>P\<^isub>e\<^isub>r\<^isub>s\<^isub>o\<^isub>n3_def X\<^isub>P\<^isub>e\<^isub>r\<^isub>s\<^isub>o\<^isub>n4_def X\<^isub>P\<^isub>e\<^isub>r\<^isub>s\<^isub>o\<^isub>n5_def X\<^isub>P\<^isub>e\<^isub>r\<^isub>s\<^isub>o\<^isub>n6_def X\<^isub>P\<^isub>e\<^isub>r\<^isub>s\<^isub>o\<^isub>n7_def X\<^isub>P\<^isub>e\<^isub>r\<^isub>s\<^isub>o\<^isub>n8_def)
+  apply(subst state_update_vs_allInstances'_rec, simp, simp add: OclAny'_def
+   person1_def person2_def person3_def person4_def person5_def person6_def person7_def person8_def)
+  apply(subst state_update_vs_allInstances'_rec, simp, simp add: OclAny'_def
+   person1_def person2_def person3_def person4_def person5_def person6_def person7_def person8_def)
+  apply(subst state_update_vs_allInstances'_rec, simp, simp add: OclAny'_def
+   person1_def person2_def person3_def person4_def person5_def person6_def person7_def person8_def)
+  apply(subst state_update_vs_allInstances'_rec, simp, simp add: OclAny'_def
+   person1_def person2_def person3_def person4_def person5_def person6_def person7_def person8_def)
+  apply(subst state_update_vs_allInstances'_rec, simp, simp add: OclAny'_def
+   person1_def person2_def person3_def person4_def person5_def person6_def person7_def person8_def)
+  apply(subst state_update_vs_allInstances'_rec, simp, simp add: OclAny'_def
+   person1_def person2_def person3_def person4_def person5_def person6_def person7_def person8_def)
+  apply(subst state_update_vs_allInstances'_rec, simp, simp add: OclAny'_def
+   person1_def person2_def person3_def person4_def person5_def person6_def person7_def person8_def)
+  apply(subst state_update_vs_allInstances'_rec0)
+
+  apply(subst including_cp_all
+                                         ) prefer 4 apply(subst cp_OclIncluding[symmetric])
+  apply(subst including_cp_all[of _ _ _ "(\<sigma>\<^isub>1, \<lparr>heap = [7 \<mapsto> in\<^isub>o\<^isub>c\<^isub>l\<^isub>a\<^isub>n\<^isub>y person8],
+                    assocs = Map.empty\<rparr>)"]) prefer 4 apply(subst cp_OclIncluding[symmetric])
+  apply(subst including_cp_all[of _ _ _ "(\<sigma>\<^isub>1, \<lparr>heap = [7 \<mapsto> in\<^isub>o\<^isub>c\<^isub>l\<^isub>a\<^isub>n\<^isub>y person8, 6 \<mapsto> in\<^isub>o\<^isub>c\<^isub>l\<^isub>a\<^isub>n\<^isub>y person7],
+                    assocs = Map.empty\<rparr>)"]) prefer 4 apply(subst cp_OclIncluding[symmetric])
+  apply(subst including_cp_all[of _ _ _ "(\<sigma>\<^isub>1, \<lparr>heap = [7 \<mapsto> in\<^isub>o\<^isub>c\<^isub>l\<^isub>a\<^isub>n\<^isub>y person8, 6 \<mapsto> in\<^isub>o\<^isub>c\<^isub>l\<^isub>a\<^isub>n\<^isub>y person7, 5 \<mapsto> in\<^isub>p\<^isub>e\<^isub>r\<^isub>s\<^isub>o\<^isub>n person6],
+                    assocs = Map.empty\<rparr>)"]) prefer 4 apply(subst cp_OclIncluding[symmetric])
+  apply(subst including_cp_all[of _ _ _ "(\<sigma>\<^isub>1, \<lparr>heap = [7 \<mapsto> in\<^isub>o\<^isub>c\<^isub>l\<^isub>a\<^isub>n\<^isub>y person8, 6 \<mapsto> in\<^isub>o\<^isub>c\<^isub>l\<^isub>a\<^isub>n\<^isub>y person7, 5 \<mapsto> in\<^isub>p\<^isub>e\<^isub>r\<^isub>s\<^isub>o\<^isub>n person6, 3 \<mapsto> in\<^isub>p\<^isub>e\<^isub>r\<^isub>s\<^isub>o\<^isub>n person4],
+                    assocs = Map.empty\<rparr>)"]) prefer 4 apply(subst cp_OclIncluding[symmetric])
+  apply(subst including_cp_all[of _ _ _ "(\<sigma>\<^isub>1, \<lparr>heap = [7 \<mapsto> in\<^isub>o\<^isub>c\<^isub>l\<^isub>a\<^isub>n\<^isub>y person8, 6 \<mapsto> in\<^isub>o\<^isub>c\<^isub>l\<^isub>a\<^isub>n\<^isub>y person7, 5 \<mapsto> in\<^isub>p\<^isub>e\<^isub>r\<^isub>s\<^isub>o\<^isub>n person6, 3 \<mapsto> in\<^isub>p\<^isub>e\<^isub>r\<^isub>s\<^isub>o\<^isub>n person4, 2 \<mapsto> in\<^isub>p\<^isub>e\<^isub>r\<^isub>s\<^isub>o\<^isub>n person3],
+                    assocs = Map.empty\<rparr>)"]) prefer 4 apply(subst cp_OclIncluding[symmetric])
+  apply(subst including_cp_all[of _ _ _ "(\<sigma>\<^isub>1, \<lparr>heap = [7 \<mapsto> in\<^isub>o\<^isub>c\<^isub>l\<^isub>a\<^isub>n\<^isub>y person8, 6 \<mapsto> in\<^isub>o\<^isub>c\<^isub>l\<^isub>a\<^isub>n\<^isub>y person7, 5 \<mapsto> in\<^isub>p\<^isub>e\<^isub>r\<^isub>s\<^isub>o\<^isub>n person6, 3 \<mapsto> in\<^isub>p\<^isub>e\<^isub>r\<^isub>s\<^isub>o\<^isub>n person4, 2 \<mapsto> in\<^isub>p\<^isub>e\<^isub>r\<^isub>s\<^isub>o\<^isub>n person3, Suc 0 \<mapsto> in\<^isub>p\<^isub>e\<^isub>r\<^isub>s\<^isub>o\<^isub>n person2],
+                    assocs = Map.empty\<rparr>)"]) prefer 4 apply(subst cp_OclIncluding[symmetric])
+  apply(subst including_cp_all[of _ _ _ "(\<sigma>\<^isub>1, \<lparr>heap = [7 \<mapsto> in\<^isub>o\<^isub>c\<^isub>l\<^isub>a\<^isub>n\<^isub>y person8, 6 \<mapsto> in\<^isub>o\<^isub>c\<^isub>l\<^isub>a\<^isub>n\<^isub>y person7, 5 \<mapsto> in\<^isub>p\<^isub>e\<^isub>r\<^isub>s\<^isub>o\<^isub>n person6, 3 \<mapsto> in\<^isub>p\<^isub>e\<^isub>r\<^isub>s\<^isub>o\<^isub>n person4, 2 \<mapsto> in\<^isub>p\<^isub>e\<^isub>r\<^isub>s\<^isub>o\<^isub>n person3, Suc 0 \<mapsto> in\<^isub>p\<^isub>e\<^isub>r\<^isub>s\<^isub>o\<^isub>n person2, 0 \<mapsto> in\<^isub>p\<^isub>e\<^isub>r\<^isub>s\<^isub>o\<^isub>n person1],
+                    assocs = Map.empty\<rparr>)"]) prefer 4 apply(subst cp_OclIncluding[symmetric])
+
+  apply(simp add: OclAny'_def person1_def person2_def person3_def person4_def person5_def person6_def person7_def person8_def)
+  apply(simp_all add: is_int_def)
+  apply((rule including_cp_all, simp_all add: is_int_def)+, simp add: mtSet_def)+
+  apply(simp add: mtSet_def) apply(simp add: mtSet_def)
+ by (metis (no_types) foundation1 foundation16 mtSet_defined)
+
+ show "?thesis \<sigma>\<^isub>1"
+  apply(simp only: StrictRefEq_set StrongEq_def true_def OclValid_def)
+  apply(subst cp_valid)
+  apply(subst (1 2) eq)
+  apply(subst cp_valid[symmetric])
+  apply(simp add: X\<^isub>P\<^isub>e\<^isub>r\<^isub>s\<^isub>o\<^isub>n1_def X\<^isub>P\<^isub>e\<^isub>r\<^isub>s\<^isub>o\<^isub>n2_def X\<^isub>P\<^isub>e\<^isub>r\<^isub>s\<^isub>o\<^isub>n3_def X\<^isub>P\<^isub>e\<^isub>r\<^isub>s\<^isub>o\<^isub>n4_def X\<^isub>P\<^isub>e\<^isub>r\<^isub>s\<^isub>o\<^isub>n5_def X\<^isub>P\<^isub>e\<^isub>r\<^isub>s\<^isub>o\<^isub>n6_def X\<^isub>P\<^isub>e\<^isub>r\<^isub>s\<^isub>o\<^isub>n7_def X\<^isub>P\<^isub>e\<^isub>r\<^isub>s\<^isub>o\<^isub>n8_def
+                  person1_def person2_def person3_def person4_def person5_def person6_def person7_def person8_def)
+ done
+qed
+
+
 
 
 lemma
